---
title: Introduction to 3D Geometry
author: Satvik Anand
date: 2024-11-05
---

## Exampler Problems 12.3

### Short Answer :

<strong>1</strong>

(i) 

![Graph(1(i))](./resources/1(i).gif)

(ii)

![Graph(1(ii))](./resources/1(ii).gif)

(iii)

![Graph(1(iii))](./resources/1(iii).gif)

(iv)

![Graph(iv)))](./resources/1(iv).gif)

<strong>2</strong>

(i) $0 : +++$

(ii) $3 : +-+$

(iii) $4 : +--$

(iv) $7 : ++-$

(v) $1 : -++$

(vi) $2 : +-+$

(vii) $4 : +--$

(viii) $6 : -+- $

<strong>3</strong>

- $(i)(3,4,2) : x(3,0,0) ; y(0,4,0) ; z(0,0,2) ;$

- $(ii)(-5,3,7) : x(-5,0,0) ; y(0,3,0) ; z(0,0,7) ;$

- $(iii)(4,-3,5) : x(4,0,0) ; y(0,-3,0) ; z(0,0,5) ;$

<strong>4</strong>

- $(i) (3,4,5) : xy(3,4,0); yz(0,4,5); zx(3,0,5);$

- $(ii) (-5,3,7) : xy(-5,3,0); yz(-5,0,7); zx(0,5,7);$

- $(iii) (4,-3,-5) : xy(4,-3,0); yz(4,0,-5); zx(0,-3,-5);$

<strong>5</strong>

Let the points be A(2,0,0) and B(-3,0,0)

Distance<sub>$(A \to B):$</sub>

$\sqrt{(x_2-x_1)^2+(y_2-y_1)^2+(z_2-z_1)^2}$

$\implies \sqrt{(-3-2)^2}$

$\implies \sqrt{25}$

$\implies 5$

<strong>6</strong>

Distance<sub>$(origin \to P):$</sub> 

$\sqrt{(x_2-x_1)^2+(y_2-y_1)^2+(z_2-z_1)^2}$

$\implies \sqrt{(6-0)^2+(6-0)^2+(7-0)^2}$

$\implies \sqrt{6^2+6^2+7^2}$

$\implies 11$

<strong>7</strong>

Given $x^2+y^2=1$ and $P(x,y,\sqrt{1-x^2-y^2})$

Distance<sub>$P \to origin$</sub>:

$\implies \sqrt{x^2+y^2+(\sqrt{1-x^2-y^2})^2}$

$\implies \sqrt{x^2+y^2+1-x^2-y^2}$

(subtracting)

$\implies \sqrt{1}$

$\implies 1$

<strong>8</strong>